src/Examples/DnsServer/DnsAutoUnify.v
@@ -12,7 +12,7 @@ Require Import
         Fiat.QueryStructure.Automation.SearchTerms.FindPrefixSearchTerms
         Fiat.QueryStructure.Automation.QSImplementation.
 
-Require Import Fiat.Examples.DnsServer.packet_new (* note use of packet_new, not DnsSchema_new *)
+Require Import Fiat.Examples.DnsServer.packet
         Fiat.Examples.DnsServer.DnsLemmas
         Fiat.Examples.DnsServer.DnsAutomation.
 
@@ -20,54 +20,51 @@ Require Import Fiat.Examples.DnsServer.DnsSchema.
 
 Definition DnsSig : ADTSig :=
   ADTsignature {
-      Constructor "Init" : unit -> rep,
-      Method "AddData" : rep x DNSRRecord -> rep x bool,
-      Method "Process" : rep x packet -> rep x packet
+      Constructor "Init" : rep,
+      Method "AddData" : rep * resourceRecord -> rep * bool,
+      Method "Process" : rep * packet -> rep * packet
     }.
+
+Open Scope ADTParsing.
 
 Definition DnsSpec : ADT DnsSig :=
   QueryADTRep DnsSchema {
-    Def Constructor "Init" (_ : unit) : rep := empty,
+    Def Constructor "Init" : rep := empty,
 
-                                               (* in start honing querystructure, it inserts constraints before every insert / decision procedure *)
-                                               (* n<- count (For (r in _) where (r = tup) return True); if n > () then.. *)
-                                               (* For refines decision procedure *)
-    update "AddData" (this : rep, t : DNSRRecord) : bool :=
+    (* in start honing querystructure, it inserts constraints before *)
+    (* every insert / decision procedure *)
+
+    Def Method1 "AddData" (this : rep) (t : resourceRecord) : rep * bool :=
       Insert t into this!sCOLLECTIONS,
 
-    query "Process" (this : rep, p : packet) : packet :=
-      let t := qtype (questions p) in
-      Repeat 1 initializing n with qname (questions p)
+    Def Method1 "Process" (this : rep) (p : packet) : rep * packet := 
+        Repeat 1 initializing n with p!"questions"!"qname"
                defaulting rec with (ret (buildempty p))
          {{ rs <- For (r in this!sCOLLECTIONS)      (* Bind a list of all the DNS entries *)
                   Where (IsPrefix r!sNAME n) (* prefixed with [n] to [rs] *)
                   (* prefix: "com.google" is a prefix of "com.google.scholar" *)
                   Return r;
-            If (negb (is_empty rs))        (* Are there any matching records? *)
-               (* TODO: this does not filter by matching QTYPE *)
-            Then
-              bfrs <- [[r in rs | upperbound name_length rs r]]; (* Find the best match (largest prefix) in [rs] *)
+            If (is_empty rs)        (* Are there any matching records? *)
+            Then ret (buildempty p) (* No matching records! *)
+            Else                (* TODO: this does not filter by matching QTYPE *)
+              (bfrs <- [[r in rs | upperbound name_length rs r]]; (* Find the best match (largest prefix) in [rs] *)
               b <- { b | decides b (forall r, List.In r bfrs -> n = r!sNAME) };
               if b                (* If the record's QNAME is an exact match  *)
               then
                 unique b,                         (* only one match (unique / otherwise) *)
                 List.In b bfrs /\ b!sTYPE = CNAME     (* If the record is a CNAME, *)
-                               /\ t <> CNAME ->>      (* and the query did not request a CNAME *)
-
+                               /\ p!"questions"!"qtype" <> CNAME ->>      (* and the query did not request a CNAME *)
                   p' <- rec b!sNAME;                  (* Recursively find records matching the CNAME *)
-                                                    (* ?? Shouldn't this use the sDATA ?? *)
-                  ret (addan p' b)
-                      (* addan : packet -> DNSRRecord -> packet *)
+                  ret (add_answer p' b)               (* ?? Shouldn't this use the sDATA ?? *)
                 otherwise ->>     (* Copy the records into the answer section of an empty response *)
                 (* multiple matches -- add them all as answers in the packet *)
-                  ret (List.fold_left addan bfrs (buildempty p))
+                  ret (List.fold_left add_answer bfrs (buildempty p))
               else              (* prefix but record's QNAME not an exact match *)
                 (* return all the prefix records that are nameserver records --
                  ask the authoritative servers *) (* TODO does this return one, or return all? *)
                 bfrs' <- [[x in bfrs | x!sTYPE = NS]];
-                ret (List.fold_left addns bfrs' (buildempty p))
-            Else ret (buildempty p) (* No matching records! *)
-          }}}.
+                ret (List.fold_left add_ns bfrs' (buildempty p)))
+          }} >>= fun p => ret (this, p)}%methDefParsing.
 
 Ltac hone_Dns :=
   start sharpening ADT;
