src/Examples/DnsServer/DnsRec.v
@@ -11,139 +11,12 @@ Require Import Fiat.QueryStructure.Automation.AutoDB
         Fiat.QueryStructure.Automation.SearchTerms.FindPrefixSearchTerms.
 
 Require Import
-        Fiat.Examples.DnsServer.packet_new
+        Fiat.Examples.DnsServer.packet
         Fiat.Examples.DnsServer.DnsLemmas.
 
 Require Import Fiat.Examples.DnsServer.DnsSchema_new.
 
 (* Only Init, MakeId, and Process should be public methods. The rest are private, for internal use. *)
-Definition DnsRecSig : ADTSig :=
-  ADTsignature {
-      Constructor "Init" : unit -> rep,
-
-      (* request state methods *)
-      Method "MakeId" : rep x name -> rep x id,
-      Method "AddRequest" : rep x (packet * id) -> rep x bool,
-      Method "GetRequestStage" : rep x id -> rep x option Stage,
-      Method "UpdateRequestStage" : rep x (id * Stage) -> rep x bool,
-
-      (* cache methods *)
-      Method "InsertResultForDomain" : rep x (time * ToStore) -> rep x bool,
-      Method "DeletePendingRequestInfo" : rep x id -> rep x bool,
-      Method "DeleteCachedNameResult" : rep x name -> rep x CacheResult,
-      Method "GetServerForLongestSuffix" : rep x (time * name) -> rep x CacheResult,
-
-      (* methods related to referrals and SLIST manipulation *)
-      Method "PacketToReferralRows" : rep x (time * packet) -> rep x list ReferralRow,
-      Method "InsertReferralRowsIntoCache" : rep x list ReferralRow -> rep x bool,
-      Method "SortSLIST" : rep x id -> rep x bool,
-      Method "ReferralRowsToSLIST" : rep x (id * name * list ReferralRow) -> rep x bool,
-      Method "GetFirstReferralAndUpdateSLIST" : rep x (time * id) -> rep x option SLIST_ReferralRow,
-      Method "UpdateCacheReferralsAndSLIST" : rep x (time * id * packet * list ReferralRow) -> rep x ToOutside,
-
-     (* TTL *)
-      Method "UpdateTTLs" : rep x time -> rep x bool,
-                                           
-      (* Main method. Talks to an outside "wrapper" in continuation-passing style. Given the time and something from the wrapper, figures out what to do with it and returns a response that may be an error, answer, or request for the wrapper to send a question to another server. *)
-      Method "Process" : rep x (time * FromOutside) -> rep x ToOutside
-    }.
-
-Variable s : list nat.
-Check [[x in s | True]].        (* Comp (list nat) -- multiple choice, over existing var s *)
-Check { x : nat | True }.   (* Comp nat -- single choice, over type nat *)
-Check { b : bool | decides b True }. (* Comp bool -- check *)
-
-(* Boilerplate to take various fields/attributes and produce a tuple.
-Should be auto-generated in newer versions of Fiat*)
-Definition Build_RequestState pac id stage :=
-  let q := questions pac in
-  < Build_Component (Build_Attribute sID nat) id,
-  Build_Component (Build_Attribute sQNAME name) (qname q),
-  Build_Component (Build_Attribute sSTAGE Stage) stage,
-  Build_Component (Build_Attribute sQTYPE RRecordType) (qtype q),
-  Build_Component (Build_Attribute sQCLASS RRecordClass) (qclass q),
-  Build_Component (Build_Attribute sPID (Bvector 16)) (id' pac),
-  Build_Component (Build_Attribute sFLAGS (Bvector 16)) (flags pac)
-  >.
-
-Definition Build_CachePointerRow reqName table :=
-  < Build_Component (Build_Attribute sDOMAIN name) reqName,
-    Build_Component (Build_Attribute sCACHETABLE CacheTable) table >.
-
-Definition Build_CacheReferralsRow tup :=
-  let '(referralDomain, rType, rClass, rTTL, serverDomain, sType, sClass, sTTL, sIP, timeLastCalculated) := tup in
-  < Build_Component (Build_Attribute sREFERRALDOMAIN name) referralDomain,
-  Build_Component (Build_Attribute sRTYPE RRecordType) rType,
-  Build_Component (Build_Attribute sRCLASS RRecordClass) rClass,
-  Build_Component (Build_Attribute sRTTL nat) rTTL,
-
-  Build_Component (Build_Attribute sSERVERDOMAIN name) serverDomain,
-  Build_Component (Build_Attribute sSTYPE RRecordType) sType,
-  Build_Component (Build_Attribute sSCLASS RRecordClass) sClass,  
-  Build_Component (Build_Attribute sSTTL nat) sTTL,
-  Build_Component (Build_Attribute sSIP name) sIP,
-  Build_Component (Build_Attribute sTIME_LAST_CALCULATED nat) timeLastCalculated >.
-
-Definition Build_CacheAnswersRow tup :=
-  let '(rDomain, rSection, rName, rType, rClass, rTTL, rRdata, timeLastCalculated) := tup in
-  < Build_Component (Build_Attribute sDOMAIN name) rDomain,
-  Build_Component (Build_Attribute sPACKET_SECTION PacketSection) rSection,
-  Build_Component (Build_Attribute sNAME name) rName,
-  Build_Component (Build_Attribute sTYPE RRecordType) rType,
-  Build_Component (Build_Attribute sCLASS RRecordClass) rClass,
-  Build_Component (Build_Attribute sTTL nat) rTTL,
-  Build_Component (Build_Attribute sRDATA name) rRdata,
-  Build_Component (Build_Attribute sTIME_LAST_CALCULATED nat) timeLastCalculated >.
-
-Definition Build_CacheFailuresRow tup :=
-  let '(rDomain, rHost, rEmail, rSerial, rRefresh, rRetry, rExpire, rMinTTL, timeLastCalculated) := tup in
-  < Build_Component (Build_Attribute sDOMAIN name) rDomain,
-  Build_Component (Build_Attribute sHOST name) rHost,
-  Build_Component (Build_Attribute sEMAIL name) rEmail,
-  Build_Component (Build_Attribute sSERIAL nat) rSerial,
-  Build_Component (Build_Attribute sREFRESH nat) rRefresh,
-  Build_Component (Build_Attribute sRETRY nat) rRetry,
-  Build_Component (Build_Attribute sEXPIRE nat) rExpire,    
-  Build_Component (Build_Attribute sMinTTL nat) rMinTTL,
-  Build_Component (Build_Attribute sTIME_LAST_CALCULATED nat) timeLastCalculated >.
-
-Definition ToSLISTRow (refRow : ReferralRow) reqId refId matchCount queryCount :=
-  < Build_Component (Build_Attribute sREQID nat) reqId,
-  Build_Component (Build_Attribute sREFERRALID nat) refId,
-  Build_Component (Build_Attribute sREFERRALDOMAIN name) refRow!sREFERRALDOMAIN,
-  Build_Component (Build_Attribute sRTYPE RRecordType) refRow!sRTYPE,
-  Build_Component (Build_Attribute sRCLASS RRecordClass) refRow!sRCLASS,
-  Build_Component (Build_Attribute sRTTL nat) refRow!sRTTL,
-
-  Build_Component (Build_Attribute sSERVERDOMAIN name) refRow!sSERVERDOMAIN,
-  Build_Component (Build_Attribute sSTYPE RRecordType) refRow!sSTYPE,
-  Build_Component (Build_Attribute sSCLASS RRecordClass) refRow!sSCLASS,  
-  Build_Component (Build_Attribute sSTTL nat) refRow!sSTTL,
-  Build_Component (Build_Attribute sSIP name) refRow!sSIP,
-  Build_Component (Build_Attribute sTIME_LAST_CALCULATED nat) refRow!sTIME_LAST_CALCULATED,
-
-  Build_Component (Build_Attribute sMATCHCOUNT nat) matchCount,
-  Build_Component (Build_Attribute sQUERYCOUNT nat) queryCount >.
-
-Definition ToSLISTOrder reqId order :=
-  < Build_Component (Build_Attribute sREQID nat) reqId,
-  Build_Component (Build_Attribute sORDER (list refPosition)) order >.
-
-Definition toPacket_soa (soa : FailureRow) : SOA :=
-  {| sourcehost := soa!sHOST;
-    contact_email := soa!sEMAIL;
-    serial := soa!sSERIAL;
-    refresh := soa!sREFRESH;
-    retry := soa!sRETRY;
-    expire := soa!sEXPIRE;
-    minTTL := soa!sMinTTL |}.
-
-Definition toPacket_ans (ans : AnswerRow) : answer :=
-  {| aname := ans!sNAME;
-    atype := ans!sTYPE;
-    aclass := ans!sCLASS;
-    ttl := ans!sTTL;
-    rdata := ans!sRDATA |}.
 
 (* So long strings of Ascii Bool Bool... won't show up in Set Printing All *)
 Definition Init := "Init".
@@ -157,12 +30,27 @@ Definition DeletePendingRequestInfo := "DeletePendingRequestInfo".
 Definition DeleteCachedNameResult := "DeleteCachedNameResult".
 Definition PacketToReferralRows :="PacketToReferralRows".
 Definition InsertReferralRowsIntoCache := "InsertReferralRowsIntoCache".
-Definition ReferralRowsToSLIST := "ReferralRowsToSLIST". 
+Definition ReferralRowsToSLIST := "ReferralRowsToSLIST".
 Definition GetFirstReferralAndUpdateSLIST := "GetFirstReferralAndUpdateSLIST".
 Definition SortSLIST := "SortSLIST".
 Definition UpdateCacheReferralsAndSLIST := "UpdateCacheReferralsAndSLIST".
 Definition UpdateTTLs := "UpdateTTLs".
 Definition Process := "Process".
+
+Definition DnsRecSig : ADTSig :=
+  ADTsignature {
+      Constructor Init : unit -> rep,
+
+      (* request state methods *)
+      Method MakeId : rep * name -> rep * id,
+
+     (* TTL *)
+      Method UpdateTTLs : rep * time -> rep * bool,
+
+      (* Main method. Talks to an outside "wrapper" in continuation-passing style. Given the time and something from the wrapper, figures out what to do with it and returns a response that may be an error, answer, or request for the wrapper to send a question to another server. *)
+      Method Process : rep * time * FromOutside -> rep * ToOutside
+    }.
+
 
 (* Helper functions *)
 
@@ -171,8 +59,8 @@ Definition upperbound' := upperbound (fun x => x).
 Definition nonempty {A : Type} (l : list A) := negb (beq_nat (List.length l) 0).
 
 (* Double the monad, double the fun! *)
-Fixpoint iterate {A B : Type} {R : RepHint} (r : repHint) (f : repHint -> A -> (Comp (repHint * B)))
-        (l : list A) : Comp (repHint * list B) :=
+Fixpoint iterate {A B : Type} {R : RepHint} (r : rep) (f : rep -> A -> (Comp (rep * B)))
+        (l : list A) : Comp (rep * list B) :=
     match l with
     | nil => ret (r, nil)
     | x :: xs =>
@@ -190,8 +78,8 @@ Definition listToOption {A : Type} (l : list A) : option A :=
   end.
 
 (* Used to join the authority and additional fields for producing a referral row *)
-Definition list_join {A B : Type} f (l1 : list A) (l2 : list B) 
-  : list (A * B) := 
+Definition list_join {A B : Type} f (l1 : list A) (l2 : list B)
+  : list (A * B) :=
   filter f (list_prod l1 l2).
 
 (* The amount of time a record has left to live (unintentionally dramatic) *)
@@ -209,431 +97,154 @@ Definition hasTimeLeft_comp TTL currTime timeLastCalculated :=
 
 (* Set Printing All. *)
 
-Definition DnsSpec_Recursive : ADT DnsRecSig :=
+
+Notation "qs ! R" :=
+  (GetRelationBnd qs {| bindex := R; indexb := _ |})
+  : QuerySpec_scope.
+
+Definition IndexedEnsemble_In
+           (U : Type) (x : U) (A : @IndexedEnsemble U) :=
+  exists idx, A {| elementIndex := idx;
+                   indexedElement := x |}.
+
+Arguments IndexedEnsemble_In [_] _ A%QuerySpec.
+
+(* Stub Methods. *)
+Definition UpdateTTLs_stub {A} (r : A) (t : time) := ret (r, false).
+
+Fixpoint InsertAll {qsSchema}
+         {A}
+         (r : QueryStructure qsSchema)
+         (idx : BoundedIndex (QSschemaNames qsSchema))
+         (rowFunc : A -> Comp _)
+         (As : list A) :=
+  (* monad iteration instead. TODO param over table *)
+  match As with
+  (* this shouldn't happen since an answer must have at >= 1 answer record *)
+  | nil => ret (r, false)
+  | a :: As' =>
+    newRow <- rowFunc a;
+    res <- QSInsert r (ibound (indexb idx)) newRow;
+      let (r'', _) := res in
+      InsertAll r'' idx rowFunc As'
+  end.
+
+Definition isQuestion (p : packet) :=
+  match p!"answers", p!"authority", p!"additional" with
+  | nil, nil, nil => true
+  | _, _, _ => false
+  end.
+
+Definition isAnswer (p : packet) := negb (is_empty (p!"answers")).
+
+Definition isReferral (p : packet) :=
+  is_empty (p!"answers")
+  && (negb (is_empty (p!"authority")))
+  && (negb (is_empty (p!"additional"))).
+Set Printing Implicit.
+
+Definition linkAuthorityAnswer (p : packet) timeArrived: list (@Tuple ReferralHeading) :=
+  let authRdataMatchesAddlName (tup2 : resourceRecord * resourceRecord) :=
+      match (fst tup2)!sRDATA with
+      | inl n => beq_name n ((snd tup2)!sNAME)
+      | _ => false
+      end in
+  let auth_addl_join := list_join authRdataMatchesAddlName (p!"authority") (p!"additional") in
+  map (fun tup_pairs : resourceRecord * resourceRecord =>
+         let (auth, addl) := tup_pairs in
+         < sREFERRALDOMAIN :: (auth!sNAME : name),
+          sRTYPE :: (auth!sTYPE : RRecordType),
+          sRCLASS :: (auth!sCLASS : RRecordClass),
+          sRTTL :: (auth!sTTL : nat),
+          (* inline RDATA and additional record *)
+          sSERVERDOMAIN :: (addl!sNAME : name),
+          sSTYPE :: (addl!sTYPE : RRecordType),
+          sSCLASS :: (addl!sCLASS : RRecordClass),
+          sSTTL :: (addl!sTTL : nat),
+          sSIP :: match (addl!sRDATA) with
+                  | inl n => n
+                  | _ => [ ]
+                  end,
+          (* IP in RDATA of additional record *)
+          sTIME_LAST_CALCULATED :: timeArrived>) auth_addl_join.
+
+(* Given a list of *new* referralrows (i.e. came from a packet, or is SBELT), *)
+(* put them in the request's SLIST, and return the current best referral. Calls many *)
+(* helper functions. *)
+
+Definition UpdateCacheReferralsAndSLISTSpec (r : QueryStructure DnsRecSchema)
+           (currTime : time) (reqId : id) (pac : packet) (referrals : list ReferralRow)
+                : Comp (_ * ToOutside) :=
+             (* Insert referrals into cache *)
+             r'' <- InsertAll r ``sCACHE_REFERRALS (fun x => ret x) referrals;
+             (* Get name of the original question *)
+             req <- For (req in (fst r'')!sREQUESTS)
+                         Where (req!sID = reqId)
+                         Return req!sQNAME;
+             match req with
+             | [ questionDomain ] =>
+               (* TODO: filter by type, class *)
+               (* Put the referrals into the request's sLIST *)
+               validReferrals <- [[ ref in referrals |
+                                    ~ exists slist_ref,
+                                        IndexedEnsemble_In slist_ref ((fst r'')!sSLIST)
+                                        /\ (ref!sREFERRALDOMAIN = slist_ref!sREFERRALDOMAIN)]];
+               r''' <- InsertAll (fst r'') ``sSLIST
+                        (fun curRef : ReferralRow =>
+                           (* Augment a referral row with the additional fields in the SLIST *)
+                           (* referral row (ids, counts) *)
+                           (* Calculate match count of referral domain to question domain *)
+                           (* e.g. ref domain = g.com, question domain = s.g.com -> count = 2 *)
+                           longestSharedSuffix <- { name' : name |
+                                                    IsPrefix name' curRef!sREFERRALDOMAIN
+                                                    /\ IsPrefix name' [""]
+                                                    /\ forall name'' : name,
+                                                        IsPrefix name'' curRef!sREFERRALDOMAIN
+                                                        -> IsPrefix name'' [""]
+                                                        -> List.length name' >= List.length name'' };
+                         (* Generate unique ids that are all greater than the existing ids *)
+                         newID <- { id : nat | forall ref,
+                                      IndexedEnsemble_In ref (r!sSLIST)
+                                      -> ref!sREQID = reqId
+                                      -> id > ref!sREFERRALID };
+                         ret (<sREQID :: reqId, sREFERRALID :: newID,
+                              sMATCHCOUNT :: (List.length longestSharedSuffix),
+                              sQUERYCOUNT :: 0 (* New Row / hasn't been queried before*) >
+                              ++ curRef))
+                        referrals;
+               (* Get the "best" referral (the one with the lowest position in SLIST), *)
+               (* add 1 to its query count, update the request's match count, and  *)
+               (* then return that "best" referral *)
+               r4 <- Update slist_ref from (fst r''')!sSLIST as slist_ref'
+                       making slist_ref'!sQUERYCOUNT = slist_ref!sQUERYCOUNT + 1
+                       where (slist_ref!sREQID = reqId /\
+                              forall slist_ref'',
+                                IndexedEnsemble_In slist_ref'' (r!sSLIST)
+                                -> slist_ref''!sMATCHCOUNT <= slist_ref!sMATCHCOUNT);
+                match r4 with
+                | (r5, bestRef :: _) =>
+                   r6 <- Update req from r5!sREQUESTS as req'
+                            making req'!sSTAGE = Some bestRef!sMATCHCOUNT
+                            where (req!sID = reqId);
+                (* Send the same question to the server with the IP given in the referral *)
+                   ret (fst r6, ServerQuestion reqId bestRef!sSIP pac)
+                | (r5, _) => ret (r5, NoReferralsLeft reqId pac)
+                end
+               | _ => ret (fst r'', NoReferralsLeft reqId pac)
+             end.
+
+Definition DnsSpec_Recursive : ADT (*DnsRecSig*) _ :=
   QueryADTRep DnsRecSchema {
-    Def Constructor Init (_ : unit) : rep := empty,
+    Def Constructor0 Init : rep := empty,
 
       (* ----- REQUESTS *)
 
       (* Generate a unique id for a request. Wrapper's responsibility to use this id for everything concerning this request and pass the correct id into functions. Requests can have (different id, same name) but not (same id, different name) since a packet can only contain one question *)
-      query MakeId (r : rep, n : name) : id :=
-        ids <- For (req in r!sREQUESTS)
-            Return (req!sID);
-        freshAscendingId <- {idx : nat | upperbound' ids idx };
-        ret freshAscendingId,
-
-        (* Uses the pre-generated id *)
-      update AddRequest (r : rep, tup : packet * id) : bool := 
-        let (pac, freshAscendingId) := tup in
-        Insert (Build_RequestState pac freshAscendingId None) into r!sREQUESTS,
-
-        (* Stage is explained in the schema file *)
-      query GetRequestStage (r : rep, reqId : id) : option Stage :=
-        stages <- For (req in r!sREQUESTS)
-            Where (reqId = req!sID)
-            Return (req!sSTAGE);
-        (* there are 0 or 1 requests matching a specific id (since unique) *)
-        ret (hd_error stages),
-
-        update UpdateRequestStage (r : rep, tup : id * Stage) : bool :=
-          let (reqId, reqStage) := tup in
-          q <- Update c from r!sREQUESTS as c'
-            making c'!sSTAGE = reqStage
-            where (c!sID = reqId);
-        let (updated, affected) := q in
-        ret (updated, nonempty affected),
-
-        (* ----- CACHE *)
-
-        (* Given a time and either an answer or a failure, convert that to the correct row type
-           and insert the rows in the correct cache table.
-        Assumes that someone has already checked that the domain is not in any of the caches. *)
-       update InsertResultForDomain (r : rep, tup : time * ToStore) : bool :=
-          let (timeArrived, toStore) := tup in
-
-          let UpdateTTLs (r : repHint) (t : time) := ret (r, false) in
-          q <- UpdateTTLs r timeArrived;
-          let (r, _) := q in
-
-          match toStore with
-          | Answer reqName pac => 
-
-            (* monad iteration instead. TODO param over table *)
-            let fix InsertAll (r' : repHint) rowFunc tups :=
-                match tups with
-                (* this shouldn't happen since an answer must have at >= 1 answer record *)
-                | nil => ret (r', false)
-                | ptup :: ptups =>
-                  res <- Insert (rowFunc ptup) into r'!sCACHE_ANSWERS;
-                  let (r'', _) := res in
-                  InsertAll r'' rowFunc ptups
-                end in
-
-            let flattenWithRec p type rec :=
-                let q := questions p in
-                (reqName, type, aname rec, atype rec, aclass rec, ttl rec, rdata rec, timeArrived) in
-            let flattenPacket p type recs := List.map (fun rec => flattenWithRec p type rec) recs in
-            let tups p := flattenPacket p PAnswer (answers p)
-                                        ++ flattenPacket p PAuthority (authority p)
-                                        ++ flattenPacket p PAdditional (additional p) in
-            res1 <- Insert (Build_CachePointerRow reqName CAnswers) into r!sCACHE_POINTERS;
-          let (r1, _) := res1 in
-          InsertAll r Build_CacheAnswersRow (tups pac)
-
-          | Failure reqName pac soa =>
-            (* ignoring authority/answer/additional fields; using only the one SOA *)
-            let mkFailTup p soa := 
-                (reqName, sourcehost soa, contact_email soa, 
-                 serial soa, refresh soa, retry soa, expire soa, minTTL soa, timeArrived) in
-            res1 <- Insert (Build_CachePointerRow reqName CFailures) into r!sCACHE_POINTERS;
-          let (r1, _) := res1 in
-          Insert (Build_CacheFailuresRow (mkFailTup pac soa)) into r1!sCACHE_FAILURES
-
-          end,
-
-          (* Delete a pending request's entry in the request's table, its SLIST order, and its SLIST *)
-          update DeletePendingRequestInfo (r : rep, reqId : id) : bool :=
-           res1 <- Delete row from r!sREQUESTS where row!sID = reqId;
-           let (r1, rows1) := res1 in
-           res2 <- Delete row from r1!sSLIST_ORDERS where row!sREQID = reqId;
-           let (r2, rows2) := res2 in
-           res3 <- Delete row from r2!sSLIST where row!sREQID = reqId;
-           let (r3, rows3) := res3 in
-           ret (r3, nonempty rows1 || nonempty rows2 || nonempty rows3),
-          
-           (* Delete a cached name's entry in the cache pointer table, as well as all relevant
-              cached answers or failures (note, does not delete things from referrals or SLIST). *)
-            update DeleteCachedNameResult (r : rep, domain : name) : CacheResult :=
-          results <- For (pointer in r!sCACHE_POINTERS)
-                   Where (pointer!sDOMAIN = domain)
-                   Return (pointer!sCACHETABLE);
-        match results with
-        (* domain to be deleted is not actually in cache *)
-        | nil => ret (r, Nope)
-        | tbl :: _ =>
-          res <- Delete row from r!sCACHE_POINTERS where row!sDOMAIN = domain;
-          let (r1, _) := res in
-          match tbl with
-          | CAnswers =>
-            answer_res <- Delete row from r1!sCACHE_ANSWERS where row!sDOMAIN = domain;
-            let (r2, ans_deleted) := answer_res in
-            ret (r2, Ans ans_deleted)
-          | CFailures =>
-              failure_res <- Delete row from r1!sCACHE_FAILURES where row!sDOMAIN = domain;
-            let (r2, fail_deleted) := failure_res in
-            ret (r2, Fail (listToOption fail_deleted))                
-          end
-        end,
-
-        (* For a given name, look in the cache and return the rows that match the longest suffix of the name. Subcase: if there already is a concrete answer/failure/referral for the name, return that. *)
-        query GetServerForLongestSuffix (r : rep, tup : time * name) : CacheResult :=
-          let (currTime, reqName) := tup in
-
-          let UpdateTTLs (r : repHint) (t : time) := ret (r, false) in
-          q <- UpdateTTLs r currTime;
-          let (r, _) := q in
-
-          let getLongestSuffixes name :=
-              (* TODO: filter by packetsection = answer? are authority/additional useful? *)
-            suffixes <- For (ans in r!sCACHE_REFERRALS)
-                Where (IsPrefix ans!sREFERRALDOMAIN name) 
-                Return ans;
-            let domainLength (tup : ReferralRow) := List.length tup!sREFERRALDOMAIN in
-            [[suffix in suffixes | upperbound domainLength suffixes suffix]] in
-
-          (* Check if we have cached results for reqName *)
-          results <- For (pointer in r!sCACHE_POINTERS)
-                   Where (pointer!sDOMAIN = reqName)
-                   Return (pointer!sCACHETABLE);
-        match results with
-        | nil =>
-          (* name has nothing cached for it, but we might have referrals for subdomains *)
-          longestSuffixes <- getLongestSuffixes reqName;
-          match longestSuffixes with
-          | _ :: _ =>
-            (* TTL* *)
-            ret (Ref longestSuffixes)
-          | nil => 
-          (* assuming prefix/subdomain failure does not imply domain failure.
-             e.g. s.com fails -/-> c.s.com fails *)
-            ret Nope (* this name has nothing cached for it *)
-          end
-          
-        | table :: _ => 
-          match table with
-                              
-          | CFailures => 
-            (* This domain [s.g.com] failed. If we have any results for the longest prefix, return them
-               and label them as referrals.
-               (e.g. an answer for [g.com]) Otherwise, return failure. *)
-            longestSuffixes <- getLongestSuffixes reqName;
-            match longestSuffixes with
-            | _ :: _ => ret (Ref longestSuffixes)
-            | nil =>
-              (* There should be only one row in Failures, containing the SOA record *)
-              nameRes <- For (f in r!sCACHE_FAILURES)
-                      Where (f!sDOMAIN = reqName)
-                      Return f;
-              (* TTL* *)
-              ret (Fail (listToOption nameRes))
-          
-            (* There may be multiple rows in Answers, containing various answer/authority/addl *)
-            (* This returns all of them and leaves it to Process to hierarchize/query them *)
-            (* (they should all be for the same domain though; the longest suffix is unique *)
-            end
-
-          | CAnswers => 
-            (* There may be multiple rows in Answers, containing various answer/authority/addl *)
-            (* This returns all of them and leaves it to Process to hierarchize/query them *)
-            nameRes <- For (f in r!sCACHE_ANSWERS)
-                    Where (f!sDOMAIN = reqName)
-                    Return f;
-            (* TTL* *)
-            ret (Ans nameRes)
-          end
-        end,
-          
-        (* -------- REFERRAL/SLIST FUNCTIONS *)
-
-        (* Does a join on the authority and additional fields of a referral-containing packet to de-hierarchize it into rows. For an example, see RFC 1034, page 47. *)
-     query PacketToReferralRows (r : rep, tup : time * packet) : list ReferralRow :=
-          let (timeArrived, pac) := tup in
-
-          let UpdateTTLs (r : repHint) (t : time) := ret (r, false) in
-          q <- UpdateTTLs r timeArrived;
-          let (r, _) := q in
-
-          (* link authority and additional fields *)
-          (* for each auth in authority, for each addl in additional, *)
-          (*  if auth's rdata = addl's name, flatten the whole thing into a row and add it *)
-          let authRdataMatchesAddlName (tup2 : answer * answer) :=
-              let (auth, addl) := tup2 in
-              beq_name (rdata auth) (aname addl) in
-          let auth_addl_join := list_join authRdataMatchesAddlName
-                                          (authority pac) (additional pac) in
-          
-          let pairToPacketTup (tup2 : answer * answer) :=
-              let q := questions pac in
-              let (auth, addl) := tup2 in
-              (aname auth, atype auth, aclass auth, ttl auth,
-               aname addl, atype addl, aclass addl, ttl addl,
-               rdata addl, timeArrived) in
-          ret (map (fun tup2 => Build_CacheReferralsRow (pairToPacketTup tup2)) auth_addl_join),
-
-          (* Unfortunately, can't parametrize iterate by the table, so here's a specific function *)
-     update InsertReferralRowsIntoCache (r : rep, referrals : list ReferralRow) : bool :=
-            let fix InsertAll (r' : repHint) rows :=
-                match rows with
-                | nil => ret (r, false)
-                | row :: rows' =>
-                  res <- Insert row into r'!sCACHE_REFERRALS;
-                let (r'', _) := res in
-                InsertAll r'' rows'
-                end in
-            InsertAll r referrals,
-
-          (* Re-sort a particular request's SLIST by descending match count.
-             Smaller position = higher match count.
-             TODO more sophisticated sorting algorithm. right now it ignores the query count *)
-     update SortSLIST (r : rep, reqId : id) : bool :=
-              (* Get the SLIST rows first so we can have predicates on them w/o being stuck in the Comp monad *)
-          allSLISTrows <- For (ref in r!sSLIST)
-                       Where (ref!sREQID = reqId)
-                       Return ref;
-          let refIds := map (fun ref => ref!sREFERRALID) allSLISTrows in
-
-          (* Delete the order, generate the new sorted order, and insert that *)
-          res1 <- Delete row from r!sSLIST_ORDERS where row!sREQID = reqId;
-          let (r2, _) := res1 in
-          let allUnique {A : Type} l := forall (x : A) (y : A), List.In x l /\ List.In y l -> x <> y in
-          (* Get match count of each referral from SLIST and compare *)
-          let matchCountGeq id1 id2 :=
-              (* Computational version *)
-              (* let find_row_with id := *)
-              (*     find (fun (row : SLIST_ReferralRow) => beq_nat row!sREFERRALID id) allSLISTrows in *)
-              (* let ref1row := find_row_with id1 in *)
-              (* let ref2row := find_row_with id2 in *)
-              (* match ref1row, ref2row with *)
-              (* | Some ref1row', Some ref2row' => ref1row'!sMATCHCOUNT >= ref2row'!sMATCHCOUNT *)
-              (* | _, _ => False *)
-
-              (* Prop version *)
-              exists ls, 
-              (For (ref1 in r!sSLIST) (ref2 in r!sSLIST)
-                    Where (ref1!sMATCHCOUNT >= ref2!sMATCHCOUNT)
-                    Return (ref1!sREQID, ref2!sREQID)) ls /\ List.In (id1, id2) ls
-              
-               in
-          (* Permutation of the old order, with unique positions, such that referrals with a greater match count have a smaller position. Positions might not be consecutive *)
-          newOrder <- { order : list refPosition | 
-                        let orderIds := map refId order in
-                        let positions := map refPos order in
-                        Permutation orderIds refIds /\ allUnique positions /\
-                        (* TODO: factor out into pairwise predicate *)
-                        (forall (ref1 ref2 : refPosition), List.In ref1 order /\ List.In ref2 order /\
-                                          refPos ref2 > refPos ref1 ->
-                                          matchCountGeq (refId ref1) (refId ref2)) };
-          Insert (ToSLISTOrder reqId newOrder) into r2!sSLIST_ORDERS,
-
-      (* Filters referrals for the valid ones (not already in list + type, class),
-      puts referrals in SLIST table with unique id (per request), and
-      adds everything to the SLIST order and re-sorts that by match count *)
-     update ReferralRowsToSLIST (r : rep, tup : id * name * list ReferralRow) : bool :=
-          let '(reqId, questionName, referrals) := tup in
-
-          (* TODO this function occurs multiple times; parametrize over table / monad iter *)
-          let fix InsertAll (r : repHint) (ids : list nat) (rows : list SLIST_ReferralRow) 
-              : Comp (repHint * bool) :=
-              match ids, rows with
-              | nil, nil => ret (r, true)
-              | refId :: ids', SLISTrow :: rows' =>
-                res <- Insert SLISTrow into r!sSLIST;
-                let (r', _) := res in 
-                InsertAll r' ids' rows'
-              | _, _ => ret (r, false) (* impossible, each row gets an id *)
-              end in
-          
-          (* Calculate match count of referral domain to question domain *)
-          (* e.g. ref domain = g.com, question domain = s.g.com -> count = 2 *)
-          let matchCount refDomain questionName :=
-              longestSharedSuffix <-
-              { name' : name | IsPrefix name' refDomain /\ IsPrefix name' questionName /\
-                               forall name'' : name, 
-                               IsPrefix name'' refDomain /\ IsPrefix name'' questionName -> 
-                               List.length name' >= List.length name'' };
-              ret (List.length longestSharedSuffix) in
-
-          (* Augment a referral row with the additional fields in the SLIST referral row (ids, counts) *)
-          let ToSLISTrow' (r : repHint) (tup : id * ReferralRow) : Comp (repHint * SLIST_ReferralRow) :=
-              let (refId, refRow) := tup in
-              matchCount' <- matchCount refRow!sREFERRALDOMAIN questionName;
-              let queryCount := 0 in (* New referral -- hasn't been queried before *)
-              ret (r, ToSLISTRow refRow reqId refId matchCount' queryCount) in
-          
-          let SortSLIST (r : repHint) (reqId : id) : Comp (repHint * bool) :=
-              ret (r, false) in (* TODO stub *)
-
-          (* -------------------------------------- *)
-          existingRefs <- For (ref in r!sSLIST)
-                       Where True
-                       Return ref;
-        (* TODO: filter by type, class *)
-          let notAlreadyInSLIST (ref : ReferralRow) := 
-              ~ exists slist_ref, List.In slist_ref existingRefs
-                                  /\ (ref!sREFERRALDOMAIN = slist_ref!sREFERRALDOMAIN) in
-          validReferrals <- [[ ref in referrals | notAlreadyInSLIST ref ]];
-
-          (* Get existing ids. could use SLIST ordering, but that's not much less work *)
-          refIds <- For (ref in r!sSLIST)
-                         Where (ref!sREQID = reqId)
-                         Return ref!sREFERRALID;
-          (* Generate unique ids that are all greater than the existing ids *)
-          newIds <- { ids : list nat | forall (x y : nat), 
-                     List.In x refIds /\ List.In y refIds -> 
-                     x <> y /\ upperbound' refIds x /\ upperbound' refIds y 
-                     /\ List.length ids = List.length referrals };
-
-          (* Turn each referral row into an SLIST referral row, then insert all of them *)
-          res0 <- iterate r ToSLISTrow' (List.combine newIds referrals);
-          let (r0, SLISTrows) := res0 in
-          res <- InsertAll r0 newIds SLISTrows;
-          let (r1, _) := res in
-
-          SortSLIST r1 reqId,
-          
-
-      (* Get the "best" referral (the one with the lowest position in SLIST),
-      add 1 to its query count, update the request's match count, and re-sort SLIST according to this.
-      Then returns that "best" referral *)
-     update GetFirstReferralAndUpdateSLIST (r : rep, tup : time * id) : option SLIST_ReferralRow :=
-      let (currTime, reqId) := tup in
-
-      let UpdateTTLs (r : repHint) (t : time) := ret (r, false) in
-      q <- UpdateTTLs r currTime;
-      let (r, _) := q in
-
-      let SortSLIST (r : repHint) (reqId : id) : Comp (repHint * bool) :=
-          ret (r, false) in (* TODO stub *)
-
-      row <- For (order in r!sSLIST_ORDERS)
-              Where (order!sREQID = reqId)
-              Return order!sORDER;
-          match hd_error row with
-          | None => ret (r, None)
-          | Some order =>
-            match order with
-            | nil => ret (r, None)
-            | _ :: _ =>
-              (* Gets referral with highest match count (according to sorting of req's SLIST order) *)
-              refWithLowestPosition <- [[ tup in order | forall tup',
-                                            List.In tup' order -> refPos tup <= refPos tup' ]];
-            (* Now that we have the ref id, get the row corresponding to that referral *)
-              match refWithLowestPosition with
-              | nil => ret (r, None) (* not possible *)
-              | ref :: _ =>
-                let bestRefId := refId ref in
-                row <- For (ref in r!sSLIST)
-                    Where (ref!sREQID = reqId /\ ref!sREFERRALID = bestRefId)
-                    Return ref;
-              match hd_error row with
-              | None => ret (r, None)
-              | Some bestRef =>
-                (* Increment queryCount, update match count, and re-sort SLIST according to match ct*)
-                (* For now, this won't change the SLIST order, but if the sorting algo starts to include queryCount, that will change the order *)
-                res <- Update c from r!sSLIST as c'
-                       making c'!sQUERYCOUNT = c!sQUERYCOUNT + 1
-                       where (c!sREQID = reqId /\ c!sREFERRALID = bestRefId);
-              let (r1, _) := res in
-              res1 <- Update c from r1!sREQUESTS as c'
-                      making c'!sSTAGE = Some bestRef!sMATCHCOUNT
-                      where (c!sID = reqId);
-              let (r2, _) := res1 in
-
-              res2 <- SortSLIST r1 reqId;
-              let (r3, _) := res2 in
-              ret (r3, Some bestRef)
-              end
-              end
-            end
-          end,
-
-          (* Given a list of *new* referralrows (i.e. came from a packet, or is SBELT),
-             put them in the request's SLIST, and return the current best referral. Calls many
-             helper functions. *)
-     update UpdateCacheReferralsAndSLIST (r : rep, tup : time * id * packet * list ReferralRow) : ToOutside :=
-        let '(currTime, reqId, pac, rows) := tup in
-
-          let UpdateTTLs (r : repHint) (t : time) := ret (r, false) in
-          q <- UpdateTTLs r currTime;
-          let (r, _) := q in
-
-        (* Stubs for above methods. *)
-        let InsertReferralRowsIntoCache (r : repHint) (referrals : list ReferralRow) := ret (r, false) in
-        let ReferralRowsToSLIST (r : repHint) reqId questionName (referrals : list ReferralRow) := ret (r, false) in
-        let GetFirstReferralAndUpdateSLIST (r : repHint) (currTime : time) (reqId : id)
-              : Comp (repHint * option SLIST_ReferralRow) := ret (r, None) in
-
-        res <- InsertReferralRowsIntoCache r rows;
-        let (r1, _) := res in
-        (* Get name of the original question *)
-        qs <- For (req in r!sREQUESTS)
-           Where (req!sID = reqId)
-           Return req!sQNAME;
-        match hd_error qs with (* exactly one *)
-        | None => ret (r, InternalCacheError reqId pac)
-        | Some questionDomain =>
-          res1 <- ReferralRowsToSLIST r1 reqId [""] rows;
-        let (r2, _) := res1 in
-        
-        res3 <- GetFirstReferralAndUpdateSLIST r2 currTime reqId;
-        let (r3, bestReferral) := res3 in
-        match bestReferral with
-        | None => ret (r3, NoReferralsLeft reqId pac)
-        | Some bestRef => 
-          (* Send the same question to the server with the IP given in the referral *)
-          ret (r3, ServerQuestion reqId bestRef!sSIP pac)
-        end
-        end,
+      Def Method1 MakeId (r : rep) (n : name) : rep * id :=
+      (* Make this a straightforward Pick *)
+      freshAscendingId <- {idx : nat | forall n, IndexedEnsemble_In n (r!sREQUESTS)
+                                                 -> idx > n!sID };
+        ret (r, freshAscendingId),
 
         (* ---------- TTL *)
      (* Decrement the TTLs of everything and store currTime in time_last_calculated,
@@ -645,159 +256,185 @@ Definition DnsSpec_Recursive : ADT DnsRecSig :=
      As a recurrence relation:
      TTL_(n+1) = TTL_n - (time_right_now - time_last_calculated) *)
         (* TODO: store the absolute time that the record should be deleted/ignored instead (when it's first added to a table), and calculate the updated TTL again when returning it *)
-        update UpdateTTLs (r : rep, currTime : time) : bool :=
+        Def Method1 UpdateTTLs (r : rep) (currTime : time) : rep * bool :=
           (* Decrement all TTLs and set the time_last_calculated to now *)
           q <- Update c from r!sSLIST as c'
             making (c'!sTIME_LAST_CALCULATED = currTime /\
                     c'!sSTTL = timeLeft c!sSTTL currTime c!sTIME_LAST_CALCULATED)
             where True;
-          let (r, _) := q in
-
-          q <- Update c from r!sCACHE_REFERRALS as c'
+          q <- Update c from (fst q)!sCACHE_REFERRALS as c'
             making (c'!sTIME_LAST_CALCULATED = currTime /\
                     c'!sSTTL = timeLeft c!sSTTL currTime c!sTIME_LAST_CALCULATED)
             where True;
-          let (r, _) := q in
-
-          q <- Update c from r!sCACHE_ANSWERS as c'
+          q <- Update c from (fst q)!sCACHE_ANSWERS as c'
             making (c'!sTIME_LAST_CALCULATED = currTime /\
                     c'!sTTL = timeLeft c!sTTL currTime c!sTIME_LAST_CALCULATED)
             where True;
-          let (r, _) := q in
-
-          q <- Update c from r!sCACHE_FAILURES as c'
+          q <- Update c from (fst q)!sCACHE_FAILURES as c'
             making (c'!sTIME_LAST_CALCULATED = currTime /\
-                    c'!sMinTTL = timeLeft c!sMinTTL currTime c!sTIME_LAST_CALCULATED)
+                    c'!"minTTL" = timeLeft c!"minTTL" currTime c!sTIME_LAST_CALCULATED)
             where True;
-          let (r, _) := q in
-
-     (* For cache tables: get all to-be-deleted rows' names and delete those from cache pointers *)
-          tbd_ref_names <- For (c in r!sCACHE_REFERRALS)
-                        Where (c!sSTTL = 0)
-                        Return (c!sREFERRALDOMAIN);
-          tbd_ans_names <- For (c in r!sCACHE_ANSWERS)
-                        Where (c!sTTL = 0)
-                        Return (c!sDOMAIN);
-          tbd_fail_names <- For (c in r!sCACHE_FAILURES)
-                        Where (c!sMinTTL = 0)
-                        Return (c!sDOMAIN);
-          let toBeDeleted := tbd_ref_names ++ tbd_ans_names ++ tbd_fail_names in
-
-          let deleteCachePointer (r : repHint) name :=
-              q <- Delete row from r!sCACHE_POINTERS where row!sDOMAIN = name;
-              let (r, affected) := q in
-              ret (r, nonempty affected) in
-          q <- iterate r deleteCachePointer toBeDeleted;
-          let (r, _) := q in
-          
-     (* For SLIST referrals: get all to-be-deleted rows' req+ref ids and delete those from SLIST order *)
-          tbd_reqId_and_refId <- For (c in r!sSLIST)
-                        Where (c!sSTTL = 0)
-                        Return (c!sREQID, c!sREFERRALID);
-
-          let deleteReqSLISTentry (r : repHint) (tup : id * id) :=
-              let (reqId, refId') := tup in
-              q <- For (c in r!sSLIST_ORDERS)
-                Where (c!sREQID = reqId)
-                Return (c!sORDER);
-              match hd_error q with
-              | None => ret (r, false)
-              | Some order =>
-                (* Delete referral with id refId from the request's SLIST *)
-                let order_ref_deleted := filter (fun tup => negb (beq_nat (refId tup) refId')) order in
-                q <- Update c from r!sSLIST_ORDERS as c'
-                     making (c'!sORDER = order_ref_deleted)
-                     where (c!sREQID = reqId);
-                let (r, affected) := q in
-                ret (r, nonempty affected)
-              end in
-          q <- iterate r deleteReqSLISTentry tbd_reqId_and_refId;
-          let (r, _) := q in
-
           (* Delete all rows from SLIST or cache with no time left to live *)
-          q <- Delete row from r!sSLIST where row!sSTTL = 0;
-          let (r, _) := q in
-          q <- Delete row from r!sCACHE_REFERRALS where row!sSTTL = 0;
-          let (r, _) := q in
-          q <- Delete row from r!sCACHE_ANSWERS where row!sTTL = 0;
-          let (r, _) := q in
-          q <- Delete row from r!sCACHE_FAILURES where row!sMinTTL = 0;
-          let (r, _) := q in
+          q <- Delete row from (fst q)!sSLIST where row!sSTTL = 0;
+          qref <- Delete row from (fst q)!sCACHE_REFERRALS where row!sSTTL = 0;
+          qans <- Delete row from (fst qref)!sCACHE_ANSWERS where row!sTTL = 0;
+          qfail <- Delete row from (fst qans)!sCACHE_FAILURES where row!"minTTL" = 0;
+          q <- Delete row from (fst qfail)!sCACHE_POINTERS where
+          ((exists ref, List.In ref (snd qref) /\ row!sDOMAIN = ref!sREFERRALDOMAIN)
+             \/ (exists ref, List.In ref (snd qans) /\ row!sDOMAIN = ref!sDOMAIN)
+             \/ (exists ref, List.In ref (snd qfail) /\ row!sDOMAIN = ref!sDOMAIN));
 
-          ret (r, true),
+            (* For cache tables: get all to-be-deleted rows' names and delete those from cache pointers *)
+          ret (fst q, true),
 
           (* ----- MAIN METHOD *)
 
       (* Main method. Talks to an outside "wrapper" in continuation-passing style. Given the time and something from the wrapper, figures out what to do with it and returns a response that may be an error, answer, or request for the wrapper to send a question to another server. *)
           (* TODO need to inline other functions; stubs for now *)
           (* TODO rep is not threaded through in Process *)
-        update Process (r : rep, tup : time * FromOutside) : ToOutside :=
-          let SBELT := @nil ReferralRow in (* TODO add root ip *)
-          (* let AddRequest (r : repHint) (tup : packet * id) := ret (r, false) in *)
-          (* let InsertResultForDomain (r : repHint) (toStore : ToStore) := ret (r, false) in *)
-          (* let GetServerForLongestSuffix (r : repHint) (reqName : name) := ret (r, Nope) in *)
-          (* let DeleteCachedNameResult (r : repHint) (domain : name) := ret (r, Nope) in *)
-          (* let DeletePendingRequestInfo (r : repHint) (reqId : id) := ret (r, false) in *)
-          (* (* SLIST/referral stubs *) *)
-          (* let PacketToReferralRows (r : repHint) (pac : packet) := ret (r, @nil ReferralRow) in *)
-          (* let UpdateCacheReferralsAndSLIST reqId pac (r : repHint) (rows : list ReferralRow) := *)
-          (*     ret (r, InvalidQuestion 0) in *)
-          let AddRequest (tup : packet * id) := ret false in
-          let InsertResultForDomain (timeArrived : time) (toStore : ToStore) := ret false in
-          let GetServerForLongestSuffix (currTime : time) (reqName : name) := ret Nope in
-          let DeleteCachedNameResult (domain : name) := ret Nope in
-          let DeletePendingRequestInfo (reqId : id) := ret false in
-          (* SLIST/referral stubs *)
-          let PacketToReferralRows (timeArrived : time) (pac : packet) := ret (@nil ReferralRow) in
-          let UpdateCacheReferralsAndSLIST (currTime : time) reqId pac (rows : list ReferralRow) := 
-              ret (InvalidQuestion 0) in
-          
-          (* Utility functions *)
-          let isQuestion p := 
-              match answers p, authority p, additional p with
-              | nil, nil, nil => true
-              | _, _, _ => false
-              end in
-          let isAnswer p := 
-              match answers p with
-              | nil => false
-              | _ :: _ => true
-              end in
-          let isReferral p :=
-              match answers p, authority p, additional p with
-              | nil, _ :: _, _ :: _ => true
-              | _, _, _ => false
-              end
-          in
-          let GetRequestName (reqId : id) : Comp (option name) :=
-            names <- For (req in r!sREQUESTS)
-                  Where (reqId = req!sID)
-                  Return (req!sQNAME);
-            ret (hd_error names) in
+          Def Method4 Process (r : rep) (timeArrived : time)
+              (reqId : id) (pac : packet) (failure : option SOA)
+          : rep * ToOutside :=
+            let SBELT := @nil ReferralRow in (* TODO add root ip *)
 
-          let (timeArrived, fromOutside) := tup in
-          let '(reqId, pac, failure) := fromOutside in
-          let reqName := qname (questions pac) in
-
-          let UpdateTTLs (r : repHint) (t : time) := ret (r, false) in
-          q <- UpdateTTLs r timeArrived;
-          let (r, _) := q in
-
-          (* --- FUNCTION START --- *)
+            (* --- FUNCTION START --- *)
           (* Is the request pending? (Are we currently working on it?) *)
           pendingReq <- For (req in r!sREQUESTS)
-                   Where (reqId = req!sID)
-                   Return req;
+                        Where (reqId = req!sID)
+                        Return req;
           (* There should be either one or none *)
-          match hd_error pendingReq with
-          | None => 
+          Ifopt (hd_error pendingReq) as pendingReq' Then
+            (* Pending *)
+            if isQuestion pac then
+              ret (r, InvalidQuestion reqId)
+            else
+              (* Figure out if the packet is an answer, failure, or referral *)
+              (* doesn't thoroughly check for malformed packets, e.g. contains answer and failure *)
+              if isReferral pac then
+                referralRows <- ret (linkAuthorityAnswer pac timeArrived);
+                UpdateCacheReferralsAndSLISTSpec r reqId timeArrived pac referralRows
+              (* Some variety of done (since not a referral) *)
+              else
+                nm <- For (req in r!sREQUESTS)
+                      Where (reqId = req!sID)
+                      Return (req!sQNAME);
+                match nm with
+                | reqName :: _  =>
+                  (* Delete the pending request's entry in the request's table, *)
+                  (* its SLIST order, and its SLIST *)
+                  r1 <- Delete row from r!sREQUESTS where row!sID = reqId;
+                  r3 <- Delete row from (fst r1)!sSLIST where row!sREQID = reqId;
+                    (* Delete a cached name's entry in the cache pointer table, as well *)
+                  (* as all relevant cached answers or failures (note, does not delete *)
+                  (* things from referrals or SLIST). *)
+                  results <- For (pointer in (fst r3)!sCACHE_POINTERS)
+                             Where (pointer!sDOMAIN = reqName)
+                             Return (pointer!sCACHETABLE);
+                  r4 <- match results with
+                        (* domain to be deleted is not actually in cache *)
+                        | [ ] => ret (r, Nope)
+                        | tbl :: _ =>
+                          r1 <- Delete row from r!sCACHE_POINTERS where row!sDOMAIN = reqName;
+                        match tbl with
+                        | CAnswers =>
+                          answer_res <- Delete row from (fst r1)!sCACHE_ANSWERS where row!sDOMAIN = reqName;
+                        ret (fst answer_res, Ans (snd answer_res))
+                        | CFailures =>
+                          failure_res <- Delete row from (fst r1)!sCACHE_FAILURES where row!sDOMAIN = reqName;
+                        ret (fst failure_res, Fail (listToOption (snd failure_res)))
+                        end
+                        end;
+                if isAnswer pac then
+                  (* Update cache *)
+                  (* Given a time and either an answer or a failure, convert that to the *)
+                  (* correct row type and insert the rows in the correct cache table. *)
+                  (* Assumes that someone has already checked that the domain is not in any *)
+                  (* of the caches. *)
+                  r1 <- Insert <sDOMAIN :: reqName, sCACHETABLE :: CAnswers >%Tuple into (fst r4)!sCACHE_POINTERS;
+                  r2 <- InsertAll (fst r1) ``sCACHE_ANSWERS
+                     (fun ans =>
+                        ret (< sDOMAIN :: reqName,
+                             sPACKET_SECTION :: PAnswer,
+                             sTIME_LAST_CALCULATED :: timeArrived> ++ ans))
+                     (pac!"answers");
+                  r3 <- InsertAll (fst r2) ``sCACHE_ANSWERS
+                     (fun ans =>
+                        ret (< sDOMAIN :: reqName,
+                             sPACKET_SECTION :: PAuthority,
+                             sTIME_LAST_CALCULATED :: timeArrived> ++ ans))
+                     (pac!"authority");
+                  r4 <- InsertAll (fst r3) ``sCACHE_ANSWERS
+                     (fun ans =>
+                        ret (< sDOMAIN :: reqName,
+                             sPACKET_SECTION :: PAdditional,
+                             sTIME_LAST_CALCULATED :: timeArrived> ++ ans))
+                     (pac!"additional");
+                  (* Done, forward it on *)
+                  ret (fst r4, ClientAnswer reqId pac)
+                else match failure with
+                     (* Failure. Done, forward it on *)
+                     | Some soa =>
+                       (* Update cache *)
+                       r1 <- Insert <sDOMAIN :: reqName, sCACHETABLE :: CFailures > into (fst r4)!sCACHE_POINTERS;
+                     r2 <- Insert (<sDOMAIN :: reqName, sTIME_LAST_CALCULATED :: timeArrived>
+                                                  ++ soa) into (fst r1)!sCACHE_FAILURES;
+                       ret (fst r2, ClientFailure reqId pac soa)
+                     | None => ret (fst r4, MissingSOA reqId pac) (* will also result in request del *)
+                     end
+                | _ => ret (r, InvalidId reqId pac)
+                end
+          Else
             (* Not pending *)
             if negb (isQuestion pac) then (* is a referral, answer, or failure *)
               ret (r, InvalidResponse reqId)
             else
               (* But have we seen it before? *)
-              suffixResults <- GetServerForLongestSuffix timeArrived reqName;
-              match suffixResults with
+              (* For a given name, look in the cache and return the rows that match the longest suffix of the name. Subcase: if there already is a concrete answer/failure/referral for the name, return that. *)
+              let reqName := (pac!"questions"!"qname") in
+              (* Check if we have cached results for reqName *)
+              results <- For (pointer in r!sCACHE_POINTERS)
+                      Where (pointer!sDOMAIN = reqName)
+                      Return (pointer!sCACHETABLE);
+                (* TODO: filter by packetsection = answer? are authority/additional useful? *)
+                res <- (
+                                suffixes <- For (ans in r!sCACHE_REFERRALS)
+                                         Where (IsPrefix ans!sREFERRALDOMAIN reqName)
+                                         Return ans;
+                                let domainLength (tup : ReferralRow) := List.length tup!sREFERRALDOMAIN in
+                                longestSuffixes <- [[suffix in suffixes | upperbound domainLength suffixes suffix]];
+                                match results with
+                                | CAnswers :: _ =>
+                                  (* There may be multiple rows in Answers, containing various answer/authority/addl *)
+                                  (* This returns all of them and leaves it to Process to hierarchize/query them *)
+                                  (* (they should all be for the same domain though; the longest suffix is unique *)
+                                  nameRes <- For (f in r!sCACHE_ANSWERS)
+                                          Where (f!sDOMAIN = reqName)
+                                          Return f;
+                                (* TTL* *)
+                                ret (r, Ans nameRes)
+
+                                | CFailures :: _ =>
+                                  (* This domain [s.g.com] failed. If we have any results for the longest prefix, *)
+                                  (* return them and label them as referrals. (e.g. an answer for [g.com])  *)
+                                  (* Otherwise, return failure. *)
+                                  If (is_empty longestSuffixes) Then
+                                     nameRes <- For (f in r!sCACHE_FAILURES)
+                                     Where (f!sDOMAIN = reqName)
+                                     Return f;
+                                (* TTL* *)
+                                ret (r, Fail (listToOption nameRes))
+                                    Else
+                                    ret (r, Ref longestSuffixes)
+
+                                | [ ] =>
+                                  (* name has nothing cached for it, but we might have referrals for subdomains *)
+                                  If (is_empty longestSuffixes) Then
+                                     ret (r, Nope) (* this name has nothing cached for it *)
+                                     Else
+                                     ret (r, Ref longestSuffixes)
+                                end);
+                let (r, suffixResults) := res in
+                match suffixResults with
                 (* Yes we have seen it *)
                 (* TODO: we may need to modify the return packet  *)
                 | Fail failure =>
@@ -808,8 +445,8 @@ Definition DnsSpec_Recursive : ADT DnsRecSig :=
                      (* TTL* *)
                      | Some soa =>
                        ret (r, ClientFailure reqId pac (toPacket_soa soa))
-                     end                  
-                | Ans answers => 
+                     end
+                | Ans answers =>
                   (* filter out Authority and Additional *)
                   actualAns <- [[ record in answers | record!sPACKET_SECTION = PAnswer ]];
                   match actualAns with
@@ -818,60 +455,290 @@ Definition DnsSpec_Recursive : ADT DnsRecSig :=
                     (* Arbitrarily choose the first answer, put it in a packet, and return it *)
                     (* TODO: could also re-hierarchize all the answer/authority/additional into pac *)
                     (* should anything go in authority and additional? *)
-                    let pac' := add_ans (buildempty pac) (toPacket_ans ans) in
+                    let pac' := add_answer (buildempty pac) (toPacket_ans ans) in
                     ret (r, ClientAnswer reqId pac')
                   end
                 | Ref referralRows =>
                   (* Add pending request *)
-                  (* TODO thread rep properly through AddRequest and UpdateCacheReferralsAndSLIST 
+                  (* TODO thread rep properly through AddRequest and UpdateCacheReferralsAndSLIST
                      (and in Nope) *)
-                  res <- AddRequest (pac, reqId);
+                  res <- Insert (Build_RequestState pac reqId None) into r!sREQUESTS;
                   (* Initialize the SLIST with best referrals, then send a question w/ the first *)
-                  outsideResult <- UpdateCacheReferralsAndSLIST reqId timeArrived pac referralRows;
-                  ret (r, outsideResult)
+                  UpdateCacheReferralsAndSLISTSpec r reqId timeArrived pac referralRows
                 (* No we haven't seen it *)
-                | Nope => 
+                | Nope =>
                   (* Add pending request *)
-                  res <- AddRequest (pac, reqId);
+                  res <- Insert (Build_RequestState pac reqId None) into r!sREQUESTS;
                   (* Initialize the SLIST with SBELT, pick one and send a question w/ the first *)
-                  outsideResult <- UpdateCacheReferralsAndSLIST reqId timeArrived pac SBELT;
-                  ret (r, outsideResult)
-              end                
-          | Some pendingReq' => 
-            (* Pending *)
-            if isQuestion pac then
-              ret (r, InvalidQuestion reqId)
-            else
-              (* Figure out if the packet is an answer, failure, or referral *)
-              (* doesn't thoroughly check for malformed packets, e.g. contains answer and failure *)
-              if isReferral pac then
-                referralRows <- PacketToReferralRows timeArrived pac;
-                outsideResult <- UpdateCacheReferralsAndSLIST timeArrived reqId pac referralRows;
-                ret (r, outsideResult)
-              (* Some variety of done (since not a referral) *)
-              else 
-                nm <- GetRequestName reqId;
-                match nm with
-                | None => ret (r, InvalidId reqId pac)
-                | Some reqName =>
-                  _ <- DeletePendingRequestInfo reqId; (* TODO return the proper rep *)
-                  _ <- DeleteCachedNameResult reqName;
-                if isAnswer pac then
-                  (* Update cache *)
-                  _ <- InsertResultForDomain timeArrived (Answer reqName pac);
-                  (* Done, forward it on *)
-                  ret (r, ClientAnswer reqId pac)
-                else match failure with
-                     (* Failure. Done, forward it on *)
-                     | Some soa => 
-                       (* Update cache *)
-                       _ <- InsertResultForDomain timeArrived (Failure reqName pac soa);
-                       ret (r, ClientFailure reqId pac soa)
-                     | None => ret (r, MissingSOA reqId pac) (* will also result in request del *)
-                     end
-                end
+                  UpdateCacheReferralsAndSLISTSpec r reqId timeArrived pac SBELT
+
+              end }%methDefParsing.
+
+(* All the old internal methods. *)
+
+      (* Uses the pre-generated id *)
+      (*Def Method2 AddRequest (r : rep)
+          (pac : packet)
+          (freshAscendingId : id) : rep * bool :=
+          Insert (Build_RequestState pac freshAscendingId None) into r!sREQUESTS,
+
+      (* Stage is explained in the schema file *)
+        Def Method1 GetRequestStage
+            (r : rep)
+            (reqId : id)
+        : rep * option Stage :=
+          stages <- For (req in r!sREQUESTS)
+                    Where (reqId = req!sID)
+                    Return (req!sSTAGE);
+        ret (r, hd_error stages),
+        (* there are 0 or 1 requests matching a specific id (since unique) *)
+
+        Def Method2 UpdateRequestStage (r : rep)
+            (reqID : id)  (reqStage : Stage) : rep * bool :=
+          q <- Update c from r!sREQUESTS as c'
+            making c'!sSTAGE = reqStage
+            where (c!sID = reqID);
+        ret (fst q, nonempty (snd q)),
+
+        (* ----- CACHE *)
+
+        (* Given a time and either an answer or a failure, convert that to the correct row type
+           and insert the rows in the correct cache table.
+        Assumes that someone has already checked that the domain is not in any of the caches. *)
+        Def Method2 InsertResultForDomain (r : rep)
+            (timeArrived : time)
+            (toStore : ToStore) : rep * bool :=
+          q <- UpdateTTLs_stub r timeArrived;
+          let (r, _) := q in
+
+          match toStore with
+          | Answer reqName pac =>
+            r1 <- Insert <sDOMAIN :: reqName, sCACHETABLE :: CAnswers >%Tuple into r!sCACHE_POINTERS;
+          r2 <- InsertAll (fst r1) ``sCACHE_ANSWERS
+             (fun ans =>
+                ret (< sDOMAIN :: reqName,
+                sPACKET_SECTION :: PAnswer,
+                sTIME_LAST_CALCULATED :: timeArrived> ++ ans))
+             (pac!"answers");
+          r3 <- InsertAll (fst r2) ``sCACHE_ANSWERS
+             (fun ans =>
+                ret (< sDOMAIN :: reqName,
+                     sPACKET_SECTION :: PAuthority,
+                     sTIME_LAST_CALCULATED :: timeArrived> ++ ans))
+             (pac!"authority");
+          InsertAll (fst r3) ``sCACHE_ANSWERS
+                    (fun ans =>
+                       ret (< sDOMAIN :: reqName,
+                            sPACKET_SECTION :: PAdditional,
+                            sTIME_LAST_CALCULATED :: timeArrived> ++ ans))
+                    (pac!"additional")
+
+          | Failure reqName pac soa =>
+            r1 <- Insert <sDOMAIN :: reqName, sCACHETABLE :: CFailures > into r!sCACHE_POINTERS;
+            Insert (<sDOMAIN :: reqName, sTIME_LAST_CALCULATED :: timeArrived>
+                                         ++ soa) into (fst r1)!sCACHE_FAILURES
+
+          end,
+
+(* Delete a pending request's entry in the request's table, its SLIST order, and its SLIST *)
+          Def Method1 DeletePendingRequestInfo (r : rep) (reqId : id) : rep * bool :=
+           r1 <- Delete row from r!sREQUESTS where row!sID = reqId;
+           r2 <- Delete row from (fst r1)!sSLIST_ORDERS where row!sREQID = reqId;
+           r3 <- Delete row from (fst r2)!sSLIST where row!sREQID = reqId;
+           ret (fst r3, nonempty (snd r1) || nonempty (snd r2) || nonempty (snd r3)),
+
+           (* Delete a cached name's entry in the cache pointer table, as well as all relevant
+              cached answers or failures (note, does not delete things from referrals or SLIST). *)
+          Def Method1 DeleteCachedNameResult (r : rep) (domain : name) : rep * CacheResult :=
+             results <- For (pointer in r!sCACHE_POINTERS)
+                     Where (pointer!sDOMAIN = domain)
+                     Return (pointer!sCACHETABLE);
+        match results with
+        (* domain to be deleted is not actually in cache *)
+        | [ ] => ret (r, Nope)
+        | tbl :: _ =>
+          r1 <- Delete row from r!sCACHE_POINTERS where row!sDOMAIN = domain;
+          match tbl with
+          | CAnswers =>
+            answer_res <- Delete row from (fst r1)!sCACHE_ANSWERS where row!sDOMAIN = domain;
+            ret (fst answer_res, Ans (snd answer_res))
+          | CFailures =>
+              failure_res <- Delete row from (fst r1)!sCACHE_FAILURES where row!sDOMAIN = domain;
+            ret (fst failure_res, Fail (listToOption (snd failure_res)))
           end
-   }.
+        end,
+
+        (* For a given name, look in the cache and return the rows that match the longest suffix of the name. Subcase: if there already is a concrete answer/failure/referral for the name, return that. *)
+        Def Method2 GetServerForLongestSuffix (r : rep)
+            (currTime : time) (reqName : name) : rep * CacheResult :=
+          (* Update the TTLs *)
+          r' <- UpdateTTLs_stub r currTime;
+        (* Check if we have cached results for reqName *)
+          results <- For (pointer in (fst r')!sCACHE_POINTERS)
+                     Where (pointer!sDOMAIN = reqName)
+                     Return (pointer!sCACHETABLE);
+        (* TODO: filter by packetsection = answer? are authority/additional useful? *)
+          suffixes <- For (ans in (fst r')!sCACHE_REFERRALS)
+                   Where (IsPrefix ans!sREFERRALDOMAIN reqName)
+                   Return ans;
+          let domainLength (tup : ReferralRow) := List.length tup!sREFERRALDOMAIN in
+          longestSuffixes <- [[suffix in suffixes | upperbound domainLength suffixes suffix]];
+            match results with
+            | CAnswers :: _ =>
+              (* There may be multiple rows in Answers, containing various answer/authority/addl *)
+              (* This returns all of them and leaves it to Process to hierarchize/query them *)
+              (* (they should all be for the same domain though; the longest suffix is unique *)
+              nameRes <- For (f in (fst r')!sCACHE_ANSWERS)
+                         Where (f!sDOMAIN = reqName)
+                         Return f;
+                (* TTL* *)
+                ret (fst r', Ans nameRes)
+
+            | CFailures :: _ =>
+              (* This domain [s.g.com] failed. If we have any results for the longest prefix, *)
+              (* return them and label them as referrals. (e.g. an answer for [g.com])  *)
+              (* Otherwise, return failure. *)
+              If (is_empty longestSuffixes) Then
+                 nameRes <- For (f in (fst r')!sCACHE_FAILURES)
+                            Where (f!sDOMAIN = reqName)
+                            Return f;
+                (* TTL* *)
+                ret (fst r', Fail (listToOption nameRes))
+              Else
+              ret (fst r', Ref longestSuffixes)
+
+            | [ ] =>
+              (* name has nothing cached for it, but we might have referrals for subdomains *)
+              If (is_empty longestSuffixes) Then
+                 ret (fst r', Nope) (* this name has nothing cached for it *)
+              Else
+                 ret (fst r', Ref longestSuffixes)
+            end,
+
+            (* -------- REFERRAL/SLIST FUNCTIONS *)
+
+            (* Filters referrals for the valid ones (not already in list + type, class), *)
+            (* puts referrals in SLIST table with unique id (per request), and *)
+            (* adds everything to the SLIST order and re-sorts that by match count *)
+            Def Method3 ReferralRowsToSLIST (r : rep) (reqId : id)
+                (questionName : name) (referrals : list ReferralRow) : rep * bool :=
+
+              (* TODO: filter by type, class *)
+              validReferrals <- [[ ref in referrals |
+                                   ~ exists slist_ref,
+                                       IndexedEnsemble_In slist_ref (r!sSLIST)
+                                       /\ (ref!sREFERRALDOMAIN = slist_ref!sREFERRALDOMAIN)]];
+              InsertAll r ``sSLIST
+                        (fun curRef : ReferralRow =>
+                           (* Augment a referral row with the additional fields in the SLIST *)
+                           (* referral row (ids, counts) *)
+                           (* Calculate match count of referral domain to question domain *)
+                           (* e.g. ref domain = g.com, question domain = s.g.com -> count = 2 *)
+                           longestSharedSuffix <- { name' : name |
+                                                    IsPrefix name' curRef!sREFERRALDOMAIN
+                                                    /\ IsPrefix name' questionName
+                                                    /\ forall name'' : name,
+                                                        IsPrefix name'' curRef!sREFERRALDOMAIN
+                                                        -> IsPrefix name'' questionName
+                                                        -> List.length name' >= List.length name'' };
+                         (* Generate unique ids that are all greater than the existing ids *)
+                         newID <- { id : nat | forall ref,
+                                      IndexedEnsemble_In ref (r!sSLIST)%QuerySpec
+                                      -> ref!sREQID = reqId
+                                      -> id > ref!sREFERRALID };
+                         ret (<sREQID :: reqId, sREFERRALID :: newID,
+                              sMATCHCOUNT :: (List.length longestSharedSuffix),
+                              sQUERYCOUNT :: 0 (* New Row / hasn't been queried before*) >
+                              ++ curRef))
+                        referrals,
+
+              (* Get the "best" referral (the one with the highest matchCount), *)
+              (* add 1 to its query count, update the request's match count, and re-sort *)
+              (* SLIST according to this. Then returns that "best" referral *)
+              Def Method2 GetFirstReferralAndUpdateSLIST
+                  (r : rep) (curTime : time) (reqId : id)
+              : rep * (option SLIST_ReferralRow) :=
+                r' <- UpdateTTLs_stub r curTime;
+                r'' <- Update slist_ref from (fst r')!sSLIST as slist_ref'
+                       making slist_ref'!sQUERYCOUNT = slist_ref!sQUERYCOUNT + 1
+                       where (slist_ref!sREQID = reqId /\
+                              forall slist_ref'',
+                                IndexedEnsemble_In slist_ref'' (r!sSLIST)
+                                -> slist_ref''!sMATCHCOUNT <= slist_ref!sMATCHCOUNT);
+                match r'' with
+                | (r''', bestRef :: _) =>
+                   res <- Update req from r'''!sREQUESTS as req'
+                            making req'!sSTAGE = Some bestRef!sMATCHCOUNT
+                            where (req!sID = reqId);
+                   ret (fst res, Some (bestRef))
+                | (r''', _) => ret (r''', None)
+                end,
+
+          (* Given a list of *new* referralrows (i.e. came from a packet, or is SBELT),
+             put them in the request's SLIST, and return the current best referral. Calls many
+             helper functions. *)
+        Def Method4 UpdateCacheReferralsAndSLIST (r : rep)
+            (currTime : time) (reqId : id) (pac : packet) (referrals : list ReferralRow)
+                : rep * ToOutside :=
+                  r' <- UpdateTTLs_stub r currTime;
+             (* Insert referrals into cache *)
+             r'' <- InsertAll (fst r') ``sCACHE_REFERRALS (fun x => ret x) referrals;
+             (* Get name of the original question *)
+             req <- For (req in (fst r'')!sREQUESTS)
+                         Where (req!sID = reqId)
+                         Return req!sQNAME;
+             match req with
+             | [ questionDomain ] =>
+               (* TODO: filter by type, class *)
+               (* Put the referrals into the request's sLIST *)
+               validReferrals <- [[ ref in referrals |
+                                    ~ exists slist_ref,
+                                        IndexedEnsemble_In slist_ref ((fst r'')!sSLIST)
+                                        /\ (ref!sREFERRALDOMAIN = slist_ref!sREFERRALDOMAIN)]];
+               r''' <- InsertAll (fst r'') ``sSLIST
+                        (fun curRef : ReferralRow =>
+                           (* Augment a referral row with the additional fields in the SLIST *)
+                           (* referral row (ids, counts) *)
+                           (* Calculate match count of referral domain to question domain *)
+                           (* e.g. ref domain = g.com, question domain = s.g.com -> count = 2 *)
+                           longestSharedSuffix <- { name' : name |
+                                                    IsPrefix name' curRef!sREFERRALDOMAIN
+                                                    /\ IsPrefix name' [""]
+                                                    /\ forall name'' : name,
+                                                        IsPrefix name'' curRef!sREFERRALDOMAIN
+                                                        -> IsPrefix name'' [""]
+                                                        -> List.length name' >= List.length name'' };
+                         (* Generate unique ids that are all greater than the existing ids *)
+                         newID <- { id : nat | forall ref,
+                                      IndexedEnsemble_In ref (r!sSLIST)
+                                      -> ref!sREQID = reqId
+                                      -> id > ref!sREFERRALID };
+                         ret (<sREQID :: reqId, sREFERRALID :: newID,
+                              sMATCHCOUNT :: (List.length longestSharedSuffix),
+                              sQUERYCOUNT :: 0 (* New Row / hasn't been queried before*) >
+                              ++ curRef))
+                        referrals;
+               (* Get the "best" referral (the one with the lowest position in SLIST), *)
+               (* add 1 to its query count, update the request's match count, and  *)
+               (* then return that "best" referral *)
+               r4 <- Update slist_ref from (fst r''')!sSLIST as slist_ref'
+                       making slist_ref'!sQUERYCOUNT = slist_ref!sQUERYCOUNT + 1
+                       where (slist_ref!sREQID = reqId /\
+                              forall slist_ref'',
+                                IndexedEnsemble_In slist_ref'' (r!sSLIST)
+                                -> slist_ref''!sMATCHCOUNT <= slist_ref!sMATCHCOUNT);
+                match r4 with
+                | (r5, bestRef :: _) =>
+                   r6 <- Update req from r5!sREQUESTS as req'
+                            making req'!sSTAGE = Some bestRef!sMATCHCOUNT
+                            where (req!sID = reqId);
+                (* Send the same question to the server with the IP given in the referral *)
+                   ret (fst r6, ServerQuestion reqId bestRef!sSIP pac)
+                | (r5, _) => ret (r5, NoReferralsLeft reqId pac)
+                end
+               | _ => ret (fst r'', NoReferralsLeft reqId pac)
+             end, *)
+
 
 (* Set Printing All. *)
 Print DnsSpec_Recursive.
